LN/Multisorted/OperationsEq.v
@@ -1,0 +1,303 @@
+From Tealeaves Require Export
+     Util.Prelude
+     Util.EqDec_eq LN.Atom LN.AtomSet LN.Leaf
+     LN.Multisorted.Operations.
+
+From Multisorted Require Import
+     Classes.DTM
+     Theory.DTMContainer
+     Theory.DTMSchedule.
+
+Import Monoid.Notations.
+Import LN.AtomSet.Notations.
+Import Classes.SetlikeFunctor.Notations.
+Import Multisorted.Theory.DTMContainer.Notations.
+
+#[local] Open Scope tealeaves_scope.
+#[local] Open Scope tealeaves_multi_scope.
+#[local] Open Scope set_scope.
+
+Section test_notations.
+
+  Import Operations.Notations.
+
+  Context
+    (S : Type -> Type)
+    `{DTPreModule (list K) S T (mn_op := Monoid_op_list) (mn_unit := Monoid_unit_list)}
+    `{! DTM (list K) T}.
+
+  Implicit Types (l : leaf) (w : list K) (t : S leaf) (x : atom).
+
+  (** ** Identity and equality lemmas for operations *)
+  (******************************************************************************)
+  Lemma open_eq : forall k t (u1 u2 : T k leaf),
+      (forall (w : list K) (l : leaf), (w, (k, l)) ∈md t -> open_loc k u1 (w, l) = open_loc k u2 (w, l)) ->
+      t '(k | u1) = t '(k | u2).
+  Proof.
+    introv hyp. unfold open. apply kbindd_respectful. auto.
+  Qed.
+
+  Lemma open_id : forall k t u,
+      (forall w l, (w, (k, l)) ∈md t -> open_loc k u (w, l) = mret T k l) ->
+      t '(k | u) = t.
+  Proof.
+    intros. unfold open.
+    now apply (kbindd_respectful_id k).
+  Qed.
+
+  Lemma subst_eq : forall k t x u1 u2,
+      (forall l, (k, l) ∈m t -> subst_loc k x u1 l = subst_loc k x u2 l) ->
+      t '{k | x ~> u1} = t '{k | x ~> u2}.
+  Proof.
+    introv hyp. unfold subst. apply kbind_respectful. auto.
+  Qed.
+
+  Lemma subst_id : forall k t x u,
+      (forall l, (k, l) ∈m t -> subst_loc k x u l = mret T k l) ->
+      t '{k | x ~> u} = t.
+  Proof.
+    intros. unfold subst.
+    now apply kbind_respectful_id.
+  Qed.
+
+  Lemma close_eq : forall k t x y,
+      (forall w l, (w, (k, l)) ∈md t -> close_loc k x (w, l) = close_loc k y (w, l)) ->
+      '[k | x] t = '[k | y] t.
+  Proof.
+    intros. unfold close.
+    now apply (kfmapd_respectful).
+  Qed.
+
+  Lemma close_id : forall k t x,
+      (forall w l, (w, (k, l)) ∈md t -> close_loc k x (w, l) = l) ->
+      '[k | x] t = t.
+  Proof.
+    intros. unfold close.
+    now apply (kfmapd_respectful_id).
+  Qed.
+
+  (** ** Context-sensitive leaf analysis of operations *)
+  (******************************************************************************)
+
+  (** *** Opening *)
+  (******************************************************************************)
+  Lemma ind_open_iff_eq : forall k l w u t,
+      (w, (k, l)) ∈md t '(k | u) <-> exists w1 w2 l1,
+        (w1, (k, l1)) ∈md t /\ (w2, (k, l)) ∈md open_loc k u (w1, l1) /\ w = w1 ● w2.
+  Proof.
+    intros. unfold open.
+    now rewrite (ind_kbindd_eq_iff S).
+  Qed.
+
+  Lemma ind_open_iff_neq : forall k j l w u t,
+      k <> j ->
+      (w, (k, l)) ∈md t '(j | u) <-> (w, (k, l)) ∈md t \/ exists w1 w2 l1,
+          (w1, (j, l1)) ∈md t /\ (w2, (k, l)) ∈md open_loc j u (w1, l1) /\ w = w1 ● w2.
+  Proof.
+    intros. unfold open.
+    now rewrite (ind_kbindd_neq_iff S); auto.
+  Qed.
+
+  (** *** Closing *)
+  (******************************************************************************)
+  Lemma ind_close_iff_eq : forall k l w x t,
+      (w, (k, l)) ∈md '[k | x] t <-> exists l1,
+        (w, (k, l1)) ∈md t /\ close_loc k x (w, l1) = l.
+  Proof.
+    intros. unfold close.
+    Fail rewrite (ind_kfmapd_eq_iff).
+  Abort.
+
+  Lemma ind_close_iff_neq : forall k j l w x t,
+      j <> k ->
+      (w, (k, l)) ∈md '[j | x] t <-> (w, (k, l)) ∈md t.
+  Proof.
+    intros. unfold close.
+    now rewrite (ind_kfmapd_iff_neq F).
+  Qed.
+
+  (** *** Substitution *)
+  (******************************************************************************)
+  Lemma ind_subst_iff_eq : forall k w l u t x,
+      (w, (k, l)) ∈md t '{k | x ~> u} <-> exists l1 w1 w2,
+        (k, (w1, l1)) ∈md t /\ (k, (w2, l)) ∈md subst_loc k x u l1 /\ w = w1 ● w2.
+  Proof.
+    intros. unfold subst.
+    now rewrite (ind_kbind_iff_eq F T k).
+  Qed.
+
+  Lemma ind_subst_iff_neq : forall k j w l u t x,
+      k <> j ->
+      (w, (k, l)) ∈md t '{j | x ~> u} <-> (w, (k, l)) ∈md t \/ exists l1 w1 w2,
+        (j, (w1, l1)) ∈md t /\ (k, (w2, l)) ∈md subst_loc j x u l1 /\ w = w1 ● w2.
+  Proof.
+    intros. unfold subst.
+    now rewrite (ind_kbind_iff_neq F T).
+  Qed.
+
+  (** ** Context-agnostic leaf analysis of operations *)
+  (******************************************************************************)
+
+  (** *** Opening *)
+  (******************************************************************************)
+  Lemma in_open_iff_eq : forall k l u t,
+      (k, l) ∈m t '(k | u) <-> exists l1 w1,
+        (k, (w1, l1)) ∈md t /\ (k, l) ∈m open_loc k u (w1, l1).
+  Proof.
+    intros. unfold open.
+    now rewrite (in_kbindd_iff_eq F T k).
+  Qed.
+
+  Lemma in_open_iff_neq : forall k j l u t,
+      k <> j ->
+      (k, l) ∈m t '(j | u) <-> (k, l) ∈m t \/ exists l1 w1,
+          (j, (w1, l1)) ∈md t /\ (k, l) ∈m open_loc j u (w1, l1).
+  Proof.
+    intros. unfold open.
+    now rewrite (in_kbindd_iff_neq F T k j).
+  Qed.
+
+  (** *** Closing *)
+  (******************************************************************************)
+  Lemma in_close_iff_eq : forall k l x t,
+      (k, l) ∈m '[k | x] t <-> exists w l1,
+        (w, (k, l1)) ∈md t /\ close_loc k x (w, l1) = l.
+  Proof.
+    intros. unfold close.
+    now rewrite (in_kfmapd_iff_eq F).
+  Qed.
+
+  Lemma in_close_iff_neq : forall k j l x t,
+      k <> j ->
+      (k, l) ∈m '[j | x] t <-> (k, l) ∈m t.
+  Proof.
+    intros. unfold close.
+    now rewrite (in_kfmapd_iff_neq F).
+  Qed.
+
+  (** *** Substitution *)
+  (******************************************************************************)
+  Lemma in_subst_iff_eq : forall k l u t x,
+      (k, l) ∈m t '{k | x ~> u} <-> exists l1,
+        (k, l1) ∈m t /\ (k, l) ∈m subst_loc k x u l1.
+  Proof.
+    intros. unfold subst.
+    now rewrite (in_kbind_iff_eq F T t k).
+  Qed.
+
+  Lemma in_subst_iff_neq : forall k j l u t x,
+      j <> k ->
+      (k, l) ∈m t '{j | x ~> u} <-> (k, l) ∈m t \/ exists l1,
+        (j, l1) ∈m t /\ (k, l) ∈m subst_loc j x u l1.
+  Proof.
+    intros. unfold subst.
+    now rewrite (in_kbind_iff_neq F T).
+  Qed.
+
+  (** ** Properties of free variables *)
+  (******************************************************************************)
+
+  (** *** Specifications for [free] and [freeset] *)
+  (******************************************************************************)
+  Theorem in_free_iff : forall (k : K) (t : F leaf) (x : atom),
+      x ∈ free F k t <-> (k, Fr x) ∈m t.
+  Proof.
+    intros. unfold free. rewrite (in_bind_iff list). split.
+    - intros [l [lin xin]]. rewrite (in_tolistk_iff) in lin.
+      destruct l as [a|n].
+      + cbv in xin. destruct xin as [?|[]].
+        subst. now rewrite in_iff_in_mlist.
+      + cbv in xin. destruct xin as [].
+    - intros. exists (Fr x). rewrite (in_tolistk_iff).
+      rewrite <- (in_iff_in_mlist). split; [assumption| ].
+      cbv. now left.
+  Qed.
+
+  Theorem in_free_iff_T : forall (k j : K) (t : T j leaf) (x : atom),
+      x ∈ free (T j) k t <-> (k, Fr x) ∈m t.
+  Proof.
+    intros. unfold free. rewrite (in_bind_iff list). split.
+    - intros [l [lin xin]]. rewrite (in_tolistk_iff) in lin.
+      destruct l as [a|n].
+      + cbv in xin. destruct xin as [?|[]].
+        subst. now rewrite in_iff_in_mlist.
+      + cbv in xin. destruct xin as [].
+    - intros. exists (Fr x). rewrite (in_tolistk_iff).
+      rewrite <- (in_iff_in_mlist). split; [assumption| ].
+      cbv. now left.
+  Qed.
+
+  Theorem free_iff_freeset : forall (k : K) (t : F leaf) (x : atom),
+      x ∈ free F k t <-> x ∈@ freeset F k t.
+  Proof.
+    intros. unfold freeset. rewrite <- in_atoms_iff.
+    reflexivity.
+  Qed.
+
+  Theorem free_iff_freeset_T : forall (k j : K) (t : T j leaf) (x : atom),
+      x ∈ free (T j) k t <-> x ∈@ freeset (T j) k t.
+  Proof.
+    intros. unfold freeset. rewrite <- in_atoms_iff.
+    reflexivity.
+  Qed.
+
+  (** *** Opening *)
+  (******************************************************************************)
+  Local Notation "x @ < k , w > ∈ t" :=
+    (tomsetd _ t (w, (k, x))) (k at level 5, w at level 5, at level 50) : tealeaves_multi_scope.
+
+  Lemma free_open_iff_eq : forall k u t x,
+      x ∈ free F k (t '(k | u)) <-> exists l1 w,
+        l1 @ <k, w> ∈ t /\ x ∈ free (T k) k (open_loc k u (w, l1)).
+  Proof.
+    intros. rewrite in_free_iff. setoid_rewrite in_free_iff_T.
+    now rewrite in_open_iff_eq.
+  Qed.
+
+  Lemma free_open_iff_neq : forall k j u t x,
+      k <> j ->
+      x ∈ free F j (t '(k | u)) <-> x ∈ free F j t \/ exists l1 w,
+          (w, (k, l1)) ∈md t /\ x ∈ free (T k) j (open_loc k u (w, l1)).
+  Proof.
+    intros. rewrite 2(in_free_iff). setoid_rewrite in_free_iff_T.
+    now rewrite in_open_iff_neq; auto.
+  Qed.
+
+  (** *** Closing *)
+  (******************************************************************************)
+  Lemma free_close_iff_eq : forall k t x y,
+      y ∈ free F k ('[k | x] t) <-> exists w l1,
+        l1 @ <k, w> ∈ t /\ close_loc k x (w, l1) = Fr y.
+  Proof.
+    intros. rewrite in_free_iff.
+    now rewrite in_close_iff_eq.
+  Qed.
+
+  Lemma free_close_iff_neq : forall k j t x,
+      k <> j ->
+      x ∈ free F j ('[k | x] t) <-> x ∈ free F j t.
+  Proof.
+    intros. rewrite 2(in_free_iff).
+    now rewrite in_close_iff_neq; auto.
+  Qed.
+
+  (** *** Substitution *)
+  (******************************************************************************)
+  Lemma free_subst_iff_eq : forall k u t x y,
+      y ∈ free F k (t '{k | x ~> u}) <-> exists l1,
+        (k, l1) ∈m t /\ y ∈ free (T k) k (subst_loc k x u l1).
+  Proof.
+    intros. rewrite (in_free_iff). setoid_rewrite (in_free_iff_T).
+    now rewrite (in_subst_iff_eq).
+  Qed.
+
+  Lemma free_subst_iff_neq : forall j k u t x y,
+      k <> j ->
+      y ∈ free F j (t '{k | x ~> u}) <-> y ∈ free F j t \/ exists l1,
+        (k, l1) ∈m t /\ y ∈ free (T k) j (subst_loc k x u l1).
+  Proof.
+    intros. rewrite 2(in_free_iff). setoid_rewrite (in_free_iff_T).
+    now rewrite (in_subst_iff_neq); auto.
+  Qed.
+
+End LocallyNameless.
